IntmDecomp: tweak rewrite system

intm/IntmDecomp.v
@@ -10,12 +10,28 @@ Module Behavior.
 
   (** *** Decomposition *)
 
-  Program Definition rho {M N P Q A} (x : t M N A) : t P Q A :=
+  Program Definition phi {M N P Q A B} (x : t M N A) : t P Q B :=
+    {|
+      has t := has x undef;
+    |}.
+
+  Program Definition nu {M N P Q A} (x : t M N A) : t P Q A :=
     {|
       has t := (exists v, has x (val v) /\ t = val v) \/ has x undef;
     |}.
   Next Obligation.
     firstorder. subst. inversion H0. eauto.
+  Qed.
+
+  Program Definition rho {M N P Q A} (x : t M N A) : t P Q A :=
+    {|
+      has t :=
+        (exists v, has x (val v) /\ t = val v) \/
+        (has x div /\ t = div) \/
+        has x undef;
+    |}.
+  Next Obligation.
+    firstorder; subst; inversion H0; eauto.
   Qed.
 
   Program Definition mu {M N P Q A} (x : t M N A) : t P Q M :=
@@ -26,19 +42,6 @@ Module Behavior.
     firstorder. subst. inversion H0. eauto.
   Qed.
 
-  Program Definition omega {M N P Q A B} (x : t M N A) : t P Q B :=
-    {|
-      has t := (has x div /\ t = div) \/ has x undef;
-    |}.
-  Next Obligation.
-    firstorder. subst. inversion H0. eauto.
-  Qed.
-
-  Program Definition ups {M N P Q A B} (x : t M N A) : t P Q B :=
-    {|
-      has t := has x undef;
-    |}.
-
   Program Definition delta {M N A} (x : t M N A) (m : M) (n : N) : t M N A :=
     {| has t := has x (tcons m n t) |}.
   Next Obligation.
@@ -46,6 +49,23 @@ Module Behavior.
   Qed.
 
   (** *** Relational properties *)
+
+  Global Instance phi_ref :
+    Monotonic
+      (@phi)
+      (forallr -, forallr -, forallr -, forallr -, forallr -, forallr -,
+        ref ++> ref).
+  Proof.
+    firstorder.
+  Qed.
+
+  Global Instance nu_ref :
+    Monotonic
+      (@nu)
+      (forallr -, forallr -, forallr -, forallr -, forallr -, ref ++> ref).
+  Proof.
+    firstorder.
+  Qed.
 
   Global Instance rho_ref :
     Monotonic
@@ -59,24 +79,6 @@ Module Behavior.
     Monotonic
       (@mu)
       (forallr -, forallr -, forallr -, forallr -, forallr -, ref ++> ref).
-  Proof.
-    firstorder.
-  Qed.
-
-  Global Instance omega_ref :
-    Monotonic
-      (@omega)
-      (forallr -, forallr -, forallr -, forallr -, forallr -, forallr -,
-        ref ++> ref).
-  Proof.
-    firstorder.
-  Qed.
-
-  Global Instance ups_ref :
-    Monotonic
-      (@ups)
-      (forallr -, forallr -, forallr -, forallr -, forallr -, forallr -,
-        ref ++> ref).
   Proof.
     firstorder.
   Qed.
@@ -97,28 +99,27 @@ Module Behavior.
     destruct 1; firstorder subst; eauto using closed.
   Qed.
 
-  Lemma omega_decr {M N A} (x : t M N A) :
-    ref (omega x) x.
+  Lemma phi_decr {M N A} (x : t M N A) :
+    ref (phi x) x.
   Proof.
-    destruct 1; firstorder subst; eauto using closed.
+    red. cbn. eauto using closed.
   Qed.
 
+  Hint Resolve rho_decr phi_decr : monad. (* sort out *)
+
   Lemma decompose {M N A} (x : t M N A) :
-    x = (rho x \/
-         omega x \/
-         mu x >>= fun m => interact m >>= delta x m)%beh.
+    x = (rho x \/ mu x >>= fun m => interact m >>= delta x m)%beh.
   Proof.
     apply antisymmetry.
     - intros t Ht. simpl.
       destruct t; eauto 20.
-      + right. right. exists (val m). intuition eauto.
+      + right. exists (val m). intuition eauto.
         constructor. simpl. eauto.
-      + right. right. exists (val m). intuition eauto using closed.
+      + right. exists (val m). intuition eauto using closed.
         constructor. simpl. eauto.
         exists (tcons m n (val n)). intuition eauto.
     - repeat apply join_lub.
       + apply rho_decr.
-      + apply omega_decr.
       + intros t (s & [(m & Hm & Hs) | H] & Hst); subst; eauto using closed.
         inversion Hst; clear Hst; subst. simpl in H0.
         destruct H0 as (? & [? | (? & ?)] & Hst); subst.
@@ -132,8 +133,21 @@ Module Behavior.
 
   (** [ret] *)
 
+  Lemma phi_ret {M N P Q A B} (v : A) :
+    @phi M N P Q A B (ret v) = bot.
+  Proof.
+    apply antisymmetry; red; cbn; firstorder congruence.
+  Qed.
+
+  Lemma nu_ret {M N P Q A} (v : A) :
+    @nu M N P Q A (ret v) = ret v.
+  Proof.
+    apply antisymmetry; try firstorder congruence.
+    red; cbn; eauto.
+  Qed.
+
   Lemma rho_ret {M N P Q A} (v : A) :
-    rho (@ret M N A v) = @ret P Q A v.
+    @rho M N P Q A (ret v) = ret v.
   Proof.
     apply antisymmetry; red; cbn; firstorder (subst; eauto; try congruence).
   Qed.
@@ -144,32 +158,28 @@ Module Behavior.
     apply antisymmetry; red; cbn; firstorder congruence.
   Qed.
 
-  Lemma omega_ret {M N P Q A B} (v : A) :
-    @omega M N P Q A B (ret v) = bot.
-  Proof.
-    apply antisymmetry; red; cbn; firstorder congruence.
-  Qed.
-
-  Lemma ups_ret {M N P Q A B} (v : A) :
-    @ups M N P Q A B (ret v) = bot.
-  Proof.
-    apply antisymmetry; red; cbn; firstorder congruence.
-  Qed.
-
   Lemma delta_ret {M N A} (v : A) (m : M) (n : N) :
     delta (ret v) m n = bot.
   Proof.
     apply antisymmetry; firstorder congruence.
   Qed.
 
-  Hint Rewrite @rho_ret @mu_ret @omega_ret @ups_ret @delta_ret : monad.
+  Hint Rewrite @phi_ret @nu_ret @rho_ret @mu_ret @delta_ret : monad.
 
   (** [bind] *)
 
   Hint Extern 1 (has _ _) => progress cbn.
 
-  Lemma rho_bind {M N P Q A B} (x : t M N A) (f : A -> t M N B) :
-    rho (P:=P) (Q:=Q) (x >>= f) = rho x >>= fun a => rho (f a).
+  Lemma phi_bind {M N P Q A B C} (x : t M N A) (f : A -> t M N B) :
+    @phi M N P Q B C (x >>= f) = nu x >>= fun a => phi (f a).
+  Proof.
+    apply antisymmetry.
+    - intro t. firstorder subst. inversion H0; clear H0; subst; eauto 20.
+    - intro t. firstorder subst; eauto 20. inversion H0; clear H0; subst; eauto.
+  Qed.
+
+  Lemma nu_bind {M N P Q A B} (x : t M N A) (f : A -> t M N B) :
+    nu (P:=P) (Q:=Q) (x >>= f) = nu x >>= fun a => nu (f a).
   Proof.
     apply antisymmetry.
     - intros t Ht. cbn in *.
@@ -179,9 +189,21 @@ Module Behavior.
       inversion Hst; clear Hst; subst; cbn in *. firstorder.
   Qed.
 
+  Lemma rho_bind {M N P Q A B} (x : t M N A) (f : A -> t M N B) :
+    rho (P:=P) (Q:=Q) (x >>= f) = rho x >>= fun a => rho (f a).
+  Proof.
+    apply antisymmetry.
+    - intros t Ht. cbn in *.
+      destruct Ht as [(v & (s & Hs & Hsv) & Ht) |
+                      [[(s & Hs & Hsv) Ht] | (s & Hs & Hsv)]]; subst;
+      inversion Hsv; clear Hsv; subst; eauto 20.
+    - intros t (s & [(v & Hv & Hsv) | [[H Ht] | H]] & Hst); subst; cbn; eauto;
+      inversion Hst; clear Hst; subst; cbn in *; firstorder.
+  Qed.
+
   Lemma mu_bind {M N P Q A B} (x : t M N A) (f : A -> t M N B) :
     mu (P:=P) (Q:=Q) (x >>= f) =
-    join (mu x) (rho x >>= fun a => mu (f a)).
+    join (mu x) (nu x >>= fun a => mu (f a)).
   Proof.
     apply antisymmetry.
     - intros t [(m & (s & Hs & Hst) & Ht) | (s & Hs & Hst)]; subst;
@@ -192,29 +214,9 @@ Module Behavior.
         inversion Hst; clear Hst; subst. firstorder.
   Qed.
 
-  Lemma omega_bind {M N P Q A B C} (x : t M N A) (f : A -> t M N B) :
-    omega (P:=P) (Q:=Q) (B:=C) (x >>= f) =
-    join (omega x) (rho x >>= fun a => omega (f a)).
-  Proof.
-    apply antisymmetry.
-    - intros t. firstorder subst. inversion H1; clear H1; subst; eauto 20.
-      inversion H0; clear H0; subst; firstorder eauto 10.
-    - intros t. firstorder subst; eauto 10.
-      inversion H0; clear H0; subst. firstorder.
-  Qed.
-
-  Lemma ups_bind {M N P Q A B C} (x : t M N A) (f : A -> t M N B) :
-    @ups M N P Q B C (x >>= f) =
-    join (ups x) (rho x >>= fun a => ups (f a)).
-  Proof.
-    apply antisymmetry.
-    - intro t. firstorder subst. inversion H0; clear H0; subst; eauto 20.
-    - intro t. firstorder subst; eauto 20. inversion H0; clear H0; subst; eauto.
-  Qed.
-
   Lemma delta_bind {M N A B} (x : t M N A) (f : A -> t M N B) m n :
     delta (x >>= f) m n =
-    join (delta x m n >>= f) (rho x >>= fun a => delta (f a) m n).
+    join (delta x m n >>= f) (nu x >>= fun a => delta (f a) m n).
   Proof.
     apply antisymmetry.
     - intros t (s & Hs & Hst).
@@ -223,9 +225,21 @@ Module Behavior.
       subst. inversion Hst; clear Hst; subst. cbn in *. eauto.
   Qed.
 
-  Hint Rewrite @rho_bind @mu_bind @omega_bind @ups_bind @delta_bind : monad.
+  Hint Rewrite @phi_bind @nu_bind @rho_bind @mu_bind @delta_bind : monad.
 
   (** [interact] *)
+
+  Lemma phi_interact {M N P Q A} m :
+    @phi M N P Q N A (interact m) = bot.
+  Proof.
+    apply antisymmetry; firstorder congruence.
+  Qed.
+
+  Lemma nu_interact {M N P Q} m :
+    @nu M N P Q N (interact m) = bot.
+  Proof.
+    apply antisymmetry; firstorder congruence.
+  Qed.
 
   Lemma rho_interact {M N P Q} m :
     @rho M N P Q N (interact m) = bot.
@@ -238,18 +252,6 @@ Module Behavior.
   Proof.
     apply antisymmetry; try firstorder congruence.
     intros _ [ ]. eauto 10.
-  Qed.
-
-  Lemma omega_interact {M N P Q A} m :
-    @omega M N P Q N A (interact m) = bot.
-  Proof.
-    apply antisymmetry; firstorder congruence.
-  Qed.
-
-  Lemma ups_interact {M N P Q A} m :
-    @ups M N P Q N A (interact m) = bot.
-  Proof.
-    apply antisymmetry; firstorder congruence.
   Qed.
 
   Lemma delta_interact {M N} (m m' : M) (n : N) :
@@ -265,14 +267,26 @@ Module Behavior.
   Qed.
 
   Hint Rewrite
+    @phi_interact
+    @nu_interact
     @rho_interact
     @mu_interact
-    @omega_interact
-    @ups_interact
     @delta_interact
     : monad.
 
   (** [join] *)
+
+  Lemma phi_join {M N P Q A B} (x y : t M N A) :
+    @phi M N P Q A B (join x y) = join (phi x) (phi y).
+  Proof.
+    apply antisymmetry; firstorder.
+  Qed.
+
+  Lemma nu_join {M N P Q A} (x y : t M N A) :
+    @nu M N P Q A (join x y) = join (nu x) (nu y).
+  Proof.
+    apply antisymmetry; firstorder.
+  Qed.
 
   Lemma rho_join {M N P Q A} (x y : t M N A) :
     @rho M N P Q A (join x y) = join (rho x) (rho y).
@@ -286,27 +300,197 @@ Module Behavior.
     apply antisymmetry; firstorder.
   Qed.
 
-  Lemma omega_join {M N P Q A B} (x y : t M N A) :
-    @omega M N P Q A B (join x y) = join (omega x) (omega y).
-  Proof.
-    apply antisymmetry; firstorder.
-  Qed.
-
-  Lemma ups_join {M N P Q A B} (x y : t M N A) :
-    @ups M N P Q A B (join x y) = join (ups x) (ups y).
-  Proof.
-    apply antisymmetry; firstorder.
-  Qed.
-
   Lemma delta_join {M N A} (x y : t M N A) m n :
     @delta M N A (join x y) m n = join (delta x m n) (delta y m n).
   Proof.
     apply antisymmetry; firstorder.
   Qed.
 
-  Hint Rewrite @rho_join @mu_join @omega_join @ups_join @delta_join : monad.
+  Hint Rewrite @phi_join @nu_join @rho_join @mu_join @delta_join : monad.
+
+  (** [meet] *)
+
+  Lemma phi_meet {M N P Q A B} (x y : t M N A) :
+    @phi M N P Q A B (meet x y) = meet (phi x) (phi y).
+  Proof.
+    apply antisymmetry; firstorder.
+  Qed.
+
+  Lemma nu_meet {M N P Q A} (x y : t M N A) :
+    @nu M N P Q A (meet x y) = meet (nu x) (nu y).
+  Proof.
+    apply antisymmetry; firstorder subst; try congruence; eauto 10 using closed.
+  Qed.
+
+  Lemma rho_meet {M N P Q A} (x y : t M N A) :
+    @rho M N P Q A (meet x y) = meet (rho x) (rho y).
+  Proof.
+    apply antisymmetry; firstorder subst; try congruence; eauto 10 using closed.
+  Qed.
+
+  Lemma mu_meet {M N P Q A} (x y : t M N A) :
+    @mu M N P Q A (meet x y) = meet (mu x) (mu y).
+  Proof.
+    apply antisymmetry; firstorder subst; try congruence; eauto using closed.
+  Qed.
+
+  Lemma delta_meet {M N A} (x y : t M N A) m n :
+    @delta M N A (meet x y) m n = meet (delta x m n) (delta y m n).
+  Proof.
+    apply antisymmetry; firstorder.
+  Qed.
+
+  Hint Rewrite @phi_meet @nu_meet @rho_meet @mu_meet @delta_meet : monad.
+
+  (** [bot] *)
+
+  Lemma phi_bot {M N P Q A B} :
+    @phi M N P Q A B bot = bot.
+  Proof.
+    apply antisymmetry; firstorder.
+  Qed.
+
+  Lemma nu_bot {M N P Q A} :
+    @nu M N P Q A bot = bot.
+  Proof.
+    apply antisymmetry; firstorder.
+  Qed.
+
+  Lemma rho_bot {M N P Q A} :
+    @rho M N P Q A bot = bot.
+  Proof.
+    apply antisymmetry; firstorder.
+  Qed.
+
+  Lemma mu_bot {M N P Q A} :
+    @mu M N P Q A bot = bot.
+  Proof.
+    apply antisymmetry; firstorder.
+  Qed.
+
+  Lemma delta_bot {M N A} m n :
+    @delta M N A bot m n = bot.
+  Proof.
+    apply antisymmetry; firstorder.
+  Qed.
+
+  Hint Rewrite @phi_bot @nu_bot @rho_bot @mu_bot @delta_bot : monad.
+
+  (** [top] *)
+
+  Lemma phi_top {M N P Q A B} :
+    @phi M N P Q A B top = top.
+  Proof.
+    apply antisymmetry; firstorder.
+  Qed.
+
+  Lemma nu_top {M N P Q A} :
+    @nu M N P Q A top = top.
+  Proof.
+    apply antisymmetry; firstorder.
+  Qed.
+
+  Lemma rho_top {M N P Q A} :
+    @rho M N P Q A top = top.
+  Proof.
+    apply antisymmetry; firstorder.
+  Qed.
+
+  Lemma mu_top {M N P Q A} :
+    @mu M N P Q A top = top.
+  Proof.
+    apply antisymmetry; firstorder.
+  Qed.
+
+  Lemma delta_top {M N A} m n :
+    @delta M N A top m n = top.
+  Proof.
+    apply antisymmetry; firstorder.
+  Qed.
+
+  Hint Rewrite @phi_top @nu_top @rho_top @mu_top @delta_top : monad.
+
+  (** [phi] *)
+
+  Lemma phi_phi {M N P Q R S A B C} (x : t M N A) :
+    @phi P Q R S B C (@phi M N P Q A B x) = phi x.
+  Proof.
+    apply antisymmetry; firstorder congruence.
+  Qed.
+
+  Lemma nu_phi {M N P Q R S A B} (x : t M N A) :
+    @nu P Q R S B (@phi M N P Q A B x) = phi x.
+  Proof.
+    apply antisymmetry; firstorder congruence.
+  Qed.
+
+  Lemma rho_phi {M N P Q R S A B} (x : t M N A) :
+    @rho P Q R S B (@phi M N P Q A B x) = phi x.
+  Proof.
+    apply antisymmetry; firstorder congruence.
+  Qed.
+
+  Lemma mu_phi {M N P Q R S A B} (x : t M N A) :
+    @mu P Q R S B (@phi M N P Q A B x) = phi x.
+  Proof.
+    apply antisymmetry; firstorder congruence.
+  Qed.
+
+  Lemma delta_phi {M N P Q A B} (x : t M N A) m n :
+    delta (@phi M N P Q A B x) m n = phi x.
+  Proof.
+    apply antisymmetry; firstorder congruence.
+  Qed.
+
+  Hint Rewrite @phi_phi @nu_phi @rho_phi @mu_phi @delta_phi : monad.
+
+  (** [nu] *)
+
+  Lemma phi_nu {M N P Q R S A B} (x : t M N A) :
+    @phi P Q R S A B (@nu M N P Q A x) = phi x.
+  Proof.
+    apply antisymmetry; firstorder congruence.
+  Qed.
+
+  Lemma nu_nu {M N P Q R S A} (x : t M N A) :
+    @nu P Q R S A (@nu M N P Q A x) = @nu M N R S A x.
+  Proof.
+    apply antisymmetry; firstorder congruence.
+  Qed.
+
+  Lemma rho_nu {M N P Q R S A} (x : t M N A) :
+    @rho P Q R S A (@nu M N P Q A x) = @nu M N R S A x.
+  Proof.
+    apply antisymmetry; firstorder congruence.
+  Qed.
+
+  Lemma mu_nu {M N P Q R S A} (x : t M N A) :
+    @mu P Q R S A (@nu M N P Q A x) = phi x.
+  Proof.
+    apply antisymmetry; firstorder congruence.
+  Qed.
+
+  Lemma delta_nu {M N P Q A} (x : t M N A) m n :
+    delta (@nu M N P Q A x) m n = phi x.
+  Proof.
+    apply antisymmetry; firstorder congruence.
+  Qed.
+
+  Hint Rewrite @phi_nu @nu_nu @rho_nu @mu_nu @delta_nu : monad.
 
   (** [rho] *)
+
+  Lemma phi_rho {M N P Q R S A B} (x : t M N A) :
+    @phi P Q R S A B (@rho M N P Q A x) = phi x.
+  Proof.
+    apply antisymmetry; firstorder congruence.
+  Qed.
+
+  Lemma nu_rho {M N P Q R S A} (x : t M N A) :
+    @nu P Q R S A (@rho M N P Q A x) = @nu M N R S A x.
+  Proof.
+    apply antisymmetry; firstorder congruence.
+  Qed.
 
   Lemma rho_rho {M N P Q R S A} (x : t M N A) :
     @rho P Q R S A (@rho M N P Q A x) = @rho M N R S A x.
@@ -315,32 +499,32 @@ Module Behavior.
   Qed.
 
   Lemma mu_rho {M N P Q R S A} (x : t M N A) :
-    @mu P Q R S A (@rho M N P Q A x) = ups x.
-  Proof.
-    apply antisymmetry; firstorder congruence.
-  Qed.
-
-  Lemma omega_rho {M N P Q R S A B} (x : t M N A) :
-    @omega P Q R S A B (@rho M N P Q A x) = ups x.
-  Proof.
-    apply antisymmetry; firstorder congruence.
-  Qed.
-
-  Lemma ups_rho {M N P Q R S A B} (x : t M N A) :
-    @ups P Q R S A B (@rho M N P Q A x) = ups x.
+    @mu P Q R S A (@rho M N P Q A x) = phi x.
   Proof.
     apply antisymmetry; firstorder congruence.
   Qed.
 
   Lemma delta_rho {M N P Q A} (x : t M N A) m n :
-    delta (@rho M N P Q A x) m n = ups x.
+    delta (@rho M N P Q A x) m n = phi x.
   Proof.
     apply antisymmetry; firstorder congruence.
   Qed.
 
-  Hint Rewrite @rho_rho @mu_rho @omega_rho @ups_rho @delta_rho : monad.
+  Hint Rewrite @phi_rho @nu_rho @rho_rho @mu_rho @delta_rho : monad.
 
   (** [mu] *)
+
+  Lemma phi_mu {M N P Q R S A} (x : t M N A) :
+    @phi P Q R S M A (@mu M N P Q A x) = phi x.
+  Proof.
+    apply antisymmetry; firstorder congruence.
+  Qed.
+
+  Lemma nu_mu {M N P Q R S A} (x : t M N A) :
+    @nu P Q R S M (@mu M N P Q A x) = mu x.
+  Proof.
+    apply antisymmetry; firstorder congruence.
+  Qed.
 
   Lemma rho_mu {M N P Q R S A} (x : t M N A) :
     @rho P Q R S M (@mu M N P Q A x) = mu x.
@@ -349,101 +533,51 @@ Module Behavior.
   Qed.
 
   Lemma mu_mu {M N P Q R S A} (x : t M N A) :
-    @mu P Q R S M (@mu M N P Q A x) = ups x.
-  Proof.
-    apply antisymmetry; firstorder congruence.
-  Qed.
-
-  Lemma omega_mu {M N P Q R S A B} (x : t M N A) :
-    @omega P Q R S M B (@mu M N P Q A x) = ups x.
-  Proof.
-    apply antisymmetry; firstorder congruence.
-  Qed.
-
-  Lemma ups_mu {M N P Q R S A} (x : t M N A) :
-    @ups P Q R S M A (@mu M N P Q A x) = ups x.
+    @mu P Q R S M (@mu M N P Q A x) = phi x.
   Proof.
     apply antisymmetry; firstorder congruence.
   Qed.
 
   Lemma delta_mu {M N P Q A} x m n :
-    delta (@mu M N P Q A x) m n = ups x.
+    delta (@mu M N P Q A x) m n = phi x.
   Proof.
     apply antisymmetry; firstorder congruence.
   Qed.
 
-  Hint Rewrite @rho_mu @mu_mu @omega_mu @ups_mu @delta_mu : monad.
-
-  (** [omega] *)
-
-  Lemma rho_omega {M N P Q R S A B} (x : t M N A) :
-    @rho P Q R S B (@omega M N P Q A B x) = ups x.
-  Proof.
-    apply antisymmetry; firstorder congruence.
-  Qed.
-
-  Lemma mu_omega {M N P Q R S A B} (x : t M N A) :
-    @mu P Q R S B (@omega M N P Q A B x) = ups x.
-  Proof.
-    apply antisymmetry; firstorder congruence.
-  Qed.
-
-  Lemma omega_omega {M N P Q R S A B C} (x : t M N A) :
-    @omega P Q R S B C (@omega M N P Q A B x) = omega x.
-  Proof.
-    apply antisymmetry; firstorder congruence.
-  Qed.
-
-  Lemma ups_omega {M N P Q R S A B C} (x : t M N A) :
-    @ups P Q R S B C (@omega M N P Q A B x) = ups x.
-  Proof.
-    apply antisymmetry; firstorder congruence.
-  Qed.
-
-  Lemma delta_omega {M N P Q A B} x m n :
-    delta (@omega M N P Q A B x) m n = ups x.
-  Proof.
-    apply antisymmetry; firstorder congruence.
-  Qed.
-
-  Hint Rewrite @rho_omega @mu_omega @omega_omega @ups_omega @delta_omega : monad.
-
-
-
+  Hint Rewrite @phi_mu @nu_mu @rho_mu @mu_mu @delta_mu : monad.
 
   (** Bind and bot *)
 
-  Lemma bind_mu_bot {M N P Q A B} x :
-    (@mu M N P Q A x >>= fun _ => @bot P Q B) = ups x.
+  Lemma bind_phi {M N P Q A B C} (x : t M N A) (f : B -> t P Q C) :
+    (phi x >>= f) = phi x.
+  Proof.
+    apply antisymmetry; intro; firstorder. eauto 10.
+  Qed.
+
+  Lemma bind_nu_bot {M N P Q A B} (x : t M N A) :
+    (nu x >>= fun _ => @bot P Q B) = phi x.
   Proof.
     apply antisymmetry; intro; firstorder subst.
     - inversion H0; contradiction.
     - cbn in *. eauto.
   Qed.
 
-  Hint Rewrite @bind_mu_bot : monad.
+  Lemma bind_mu_bot {M N P Q A B} (x : t M N A) :
+    (mu x >>= fun _ => @bot P Q B) = phi x.
+  Proof.
+    apply antisymmetry; intro; firstorder subst.
+    - inversion H0; contradiction.
+    - cbn in *. eauto.
+  Qed.
 
+  Hint Rewrite @bind_phi @bind_nu_bot @bind_mu_bot : monad.
+
+End Behavior.
+
+(*
 Global Instance subrel_subrelation {A} (R R' : relation A) :
   RAuto (subrel R R') -> subrelation R R'.
 Proof.
   firstorder.
 Qed.
-
-
-  Lemma bind_ups {M N P Q A B C} (x : t M N A) (f : B -> t P Q C) :
-    ups x >>= f = ups x.
-  Proof.
-    apply antisymmetry; firstorder eauto 10.
-  Qed.
-
-  Hint Rewrite @bind_ups : monad.
-
-  Lemma ups_decr {M N A} (x : t M N A) :
-    ref (ups x) x.
-  Proof.
-    red. cbn. eauto using closed.
-  Qed.
-
-  Hint Resolve ups_decr : monad.
-
-End Behavior.
+*)
